theories/algebra/iprod.v
@@ -1,15 +1,18 @@
 From iris.algebra Require Export cmra.
-From iris.base_logic Require Import base_logic.
+From iris.algebra Require Import updates.
 From stdpp Require Import finite.
 Set Default Proof Using "Type".
 
-(** * Indexed product *)
 Definition iprod_insert `{EqDecision A} {B : A → ofeT}
-    (x : A) (y : B x) (f : iprodC B) : iprodC B := λ x',
+    (x : A) (y : B x) (f : iprod B) : iprod B := λ x',
   match decide (x = x') with left H => eq_rect _ B y _ H | right _ => f x' end.
 Instance: Params (@iprod_insert) 5.
 
-Section iprod_operations.
+Definition iprod_singleton `{Finite A} {B : A → ucmraT} 
+  (x : A) (y : B x) : iprod B := iprod_insert x y ε.
+Instance: Params (@iprod_singleton) 5.
+
+Section ofe.
   Context `{Heqdec : EqDecision A} {B : A → ofeT}.
   Implicit Types x : A.
   Implicit Types f g : iprod B.
@@ -33,14 +36,6 @@ Section iprod_operations.
     x ≠ x' → (iprod_insert x y f) x' = f x'.
   Proof. by rewrite /iprod_insert; destruct (decide _). Qed.
 
-  Global Instance iprod_lookup_discrete f x : Discrete f → Discrete (f x).
-  Proof using Heqdec.
-    intros ? y ?.
-    cut (f ≡ iprod_insert x y f).
-    { by move=> /(_ x)->; rewrite iprod_lookup_insert. }
-    apply (discrete _)=> x'; destruct (decide (x = x')) as [->|];
-      by rewrite ?iprod_lookup_insert ?iprod_lookup_insert_ne.
-  Qed.
   Global Instance iprod_insert_discrete f x y :
     Discrete f → Discrete y → Discrete (iprod_insert x y f).
   Proof.
@@ -50,111 +45,12 @@ Section iprod_operations.
     - rewrite iprod_lookup_insert_ne //.
       apply: discrete. by rewrite -(Heq x') iprod_lookup_insert_ne.
   Qed.
-End iprod_operations.
+End ofe.
 
-Section iprod_cmra.
-  Context `{Hfin : Finite A} {B : A → ucmraT}.
-  Implicit Types f g : iprod B.
-
-  Instance iprod_op : Op (iprod B) := λ f g x, f x ⋅ g x.
-  Instance iprod_pcore : PCore (iprod B) := λ f, Some (λ x, core (f x)).
-  Instance iprod_valid : Valid (iprod B) := λ f, ∀ x, ✓ f x.
-  Instance iprod_validN : ValidN (iprod B) := λ n f, ∀ x, ✓{n} f x.
-
-  Definition iprod_lookup_op f g x : (f ⋅ g) x = f x ⋅ g x := eq_refl.
-  Definition iprod_lookup_core f x : (core f) x = core (f x) := eq_refl.
-
-  Lemma iprod_included_spec (f g : iprod B) : f ≼ g ↔ ∀ x, f x ≼ g x.
-  Proof using Hfin.
-    split; [by intros [h Hh] x; exists (h x); rewrite /op /iprod_op (Hh x)|].
-    intros [h ?]%finite_choice. by exists h.
-  Qed.
-
-  Lemma iprod_cmra_mixin : CmraMixin (iprod B).
-  Proof using Hfin.
-    apply cmra_total_mixin.
-    - eauto.
-    - by intros n f1 f2 f3 Hf x; rewrite iprod_lookup_op (Hf x).
-    - by intros n f1 f2 Hf x; rewrite iprod_lookup_core (Hf x).
-    - by intros n f1 f2 Hf ? x; rewrite -(Hf x).
-    - intros g; split.
-      + intros Hg n i; apply cmra_valid_validN, Hg.
-      + intros Hg i; apply cmra_valid_validN=> n; apply Hg.
-    - intros n f Hf x; apply cmra_validN_S, Hf.
-    - by intros f1 f2 f3 x; rewrite iprod_lookup_op assoc.
-    - by intros f1 f2 x; rewrite iprod_lookup_op comm.
-    - by intros f x; rewrite iprod_lookup_op iprod_lookup_core cmra_core_l.
-    - by intros f x; rewrite iprod_lookup_core cmra_core_idemp.
-    - intros f1 f2; rewrite !iprod_included_spec=> Hf x.
-      by rewrite iprod_lookup_core; apply cmra_core_mono, Hf.
-    - intros n f1 f2 Hf x; apply cmra_validN_op_l with (f2 x), Hf.
-    - intros n f f1 f2 Hf Hf12.
-      destruct (finite_choice (λ x (yy : B x * B x),
-        f x ≡ yy.1 ⋅ yy.2 ∧ yy.1 ≡{n}≡ f1 x ∧ yy.2 ≡{n}≡ f2 x)) as [gg Hgg].
-      { intros x. specialize (Hf12 x).
-        destruct (cmra_extend n (f x) (f1 x) (f2 x)) as (y1&y2&?&?&?); eauto.
-        exists (y1,y2); eauto. }
-      exists (λ x, gg x.1), (λ x, gg x.2). split_and!=> -?; naive_solver.
-  Qed.
-  Canonical Structure iprodR := CmraT (iprod B) iprod_cmra_mixin.
-
-  Instance iprod_unit : Unit (iprod B) := λ x, ε.
-  Definition iprod_lookup_empty x : ε x = ε := eq_refl.
-
-  Lemma iprod_ucmra_mixin : UcmraMixin (iprod B).
-  Proof.
-    split.
-    - intros x; apply ucmra_unit_valid.
-    - by intros f x; rewrite iprod_lookup_op left_id.
-    - constructor=> x. apply core_id_core, _.
-  Qed.
-  Canonical Structure iprodUR := UcmraT (iprod B) iprod_ucmra_mixin.
-
-  Global Instance iprod_unit_discrete :
-    (∀ i, Discrete (ε : B i)) → Discrete (ε : iprod B).
-  Proof. intros ? f Hf x. by apply: discrete. Qed.
-
-  (** Internalized properties *)
-  Lemma iprod_equivI {M} g1 g2 : g1 ≡ g2 ⊣⊢ (∀ i, g1 i ≡ g2 i : uPred M).
-  Proof. by uPred.unseal. Qed.
-  Lemma iprod_validI {M} g : ✓ g ⊣⊢ (∀ i, ✓ g i : uPred M).
-  Proof. by uPred.unseal. Qed.
-
-  (** Properties of iprod_insert. *)
-  Lemma iprod_insert_updateP x (P : B x → Prop) (Q : iprod B → Prop) g y1 :
-    y1 ~~>: P → (∀ y2, P y2 → Q (iprod_insert x y2 g)) →
-    iprod_insert x y1 g ~~>: Q.
-  Proof.
-    intros Hy1 HP; apply cmra_total_updateP.
-    intros n gf Hg. destruct (Hy1 n (Some (gf x))) as (y2&?&?).
-    { move: (Hg x). by rewrite iprod_lookup_op iprod_lookup_insert. }
-    exists (iprod_insert x y2 g); split; [auto|].
-    intros x'; destruct (decide (x' = x)) as [->|];
-      rewrite iprod_lookup_op ?iprod_lookup_insert //; [].
-    move: (Hg x'). by rewrite iprod_lookup_op !iprod_lookup_insert_ne.
-  Qed.
-
-  Lemma iprod_insert_updateP' x (P : B x → Prop) g y1 :
-    y1 ~~>: P →
-    iprod_insert x y1 g ~~>: λ g', ∃ y2, g' = iprod_insert x y2 g ∧ P y2.
-  Proof. eauto using iprod_insert_updateP. Qed.
-  Lemma iprod_insert_update g x y1 y2 :
-    y1 ~~> y2 → iprod_insert x y1 g ~~> iprod_insert x y2 g.
-  Proof.
-    rewrite !cmra_update_updateP; eauto using iprod_insert_updateP with subst.
-  Qed.
-End iprod_cmra.
-
-Arguments iprodR {_ _ _} _.
-Arguments iprodUR {_ _ _} _.
-
-Definition iprod_singleton `{Finite A} {B : A → ucmraT} 
-  (x : A) (y : B x) : iprod B := iprod_insert x y ε.
-Instance: Params (@iprod_singleton) 5.
-
-Section iprod_singleton.
+Section cmra.
   Context `{Finite A} {B : A → ucmraT}.
   Implicit Types x : A.
+  Implicit Types f g : iprod B.
 
   Global Instance iprod_singleton_ne x :
     NonExpansive (iprod_singleton x : B x → _).
@@ -200,6 +96,29 @@ Section iprod_singleton.
     - by rewrite iprod_lookup_op !iprod_lookup_singleton_ne // left_id.
   Qed.
 
+  Lemma iprod_insert_updateP x (P : B x → Prop) (Q : iprod B → Prop) g y1 :
+    y1 ~~>: P → (∀ y2, P y2 → Q (iprod_insert x y2 g)) →
+    iprod_insert x y1 g ~~>: Q.
+  Proof.
+    intros Hy1 HP; apply cmra_total_updateP.
+    intros n gf Hg. destruct (Hy1 n (Some (gf x))) as (y2&?&?).
+    { move: (Hg x). by rewrite iprod_lookup_op iprod_lookup_insert. }
+    exists (iprod_insert x y2 g); split; [auto|].
+    intros x'; destruct (decide (x' = x)) as [->|];
+      rewrite iprod_lookup_op ?iprod_lookup_insert //; [].
+    move: (Hg x'). by rewrite iprod_lookup_op !iprod_lookup_insert_ne.
+  Qed.
+
+  Lemma iprod_insert_updateP' x (P : B x → Prop) g y1 :
+    y1 ~~>: P →
+    iprod_insert x y1 g ~~>: λ g', ∃ y2, g' = iprod_insert x y2 g ∧ P y2.
+  Proof. eauto using iprod_insert_updateP. Qed.
+  Lemma iprod_insert_update g x y1 y2 :
+    y1 ~~> y2 → iprod_insert x y1 g ~~> iprod_insert x y2 g.
+  Proof.
+    rewrite !cmra_update_updateP; eauto using iprod_insert_updateP with subst.
+  Qed.
+
   Lemma iprod_singleton_updateP x (P : B x → Prop) (Q : iprod B → Prop) y1 :
     y1 ~~>: P → (∀ y2, P y2 → Q (iprod_singleton x y2)) →
     iprod_singleton x y1 ~~>: Q.
@@ -231,38 +150,4 @@ Section iprod_singleton.
     rewrite !cmra_update_updateP;
       eauto using iprod_singleton_updateP_empty with subst.
   Qed.
-End iprod_singleton.
-
-(** * Functor *)
-Instance iprod_map_cmra_morphism
-    `{Finite A} {B1 B2 : A → ucmraT} (f : ∀ x, B1 x → B2 x) :
-  (∀ x, CmraMorphism (f x)) → CmraMorphism (iprod_map f).
-Proof.
-  split; first apply _.
-  - intros n g Hg x; rewrite /iprod_map; apply (cmra_morphism_validN (f _)), Hg.
-  - intros. apply Some_proper=>i. apply (cmra_morphism_core (f i)).
-  - intros g1 g2 i. by rewrite /iprod_map iprod_lookup_op cmra_morphism_op.
-Qed.
-
-Program Definition iprodURF `{Finite C} (F : C → urFunctor) : urFunctor := {|
-  urFunctor_car A B := iprodUR (λ c, urFunctor_car (F c) A B);
-  urFunctor_map A1 A2 B1 B2 fg := iprodC_map (λ c, urFunctor_map (F c) fg)
-|}.
-Next Obligation.
-  intros C ?? F A1 A2 B1 B2 n ?? g.
-  by apply iprodC_map_ne=>?; apply urFunctor_ne.
-Qed.
-Next Obligation.
-  intros C ?? F A B g; simpl. rewrite -{2}(iprod_map_id g).
-  apply iprod_map_ext=> y; apply urFunctor_id.
-Qed.
-Next Obligation.
-  intros C ?? F A1 A2 A3 B1 B2 B3 f1 f2 f1' f2' g. rewrite /=-iprod_map_compose.
-  apply iprod_map_ext=>y; apply urFunctor_compose.
-Qed.
-Instance iprodURF_contractive `{Finite C} (F : C → urFunctor) :
-  (∀ c, urFunctorContractive (F c)) → urFunctorContractive (iprodURF F).
-Proof.
-  intros ? A1 A2 B1 B2 n ?? g.
-  by apply iprodC_map_ne=>c; apply urFunctor_contractive.
-Qed.
+End cmra.
