theories/algebra/ofe.v
@@ -511,42 +511,6 @@ Section fixpointAB_ne.
   Proof. setoid_rewrite equiv_dist; naive_solver eauto using fixpoint_B_ne. Qed.
 End fixpointAB_ne.
 
-(** Function space *)
-(* We make [iprod] a definition so that we can register it as a canonical
-structure. *)
-Definition iprod {A} (B : A → ofeT) := ∀ x : A, B x.
-
-Section iprod.
-  Context {A : Type} {B : A → ofeT}.
-  Instance iprod_equiv : Equiv (iprod B) := λ f g, ∀ x, f x ≡ g x.
-  Instance iprod_dist : Dist (iprod B) := λ n f g, ∀ x, f x ≡{n}≡ g x.
-  Definition iprod_ofe_mixin : OfeMixin (iprod B).
-  Proof.
-    split.
-    - intros f g; split; [intros Hfg n k; apply equiv_dist, Hfg|].
-      intros Hfg k; apply equiv_dist=> n; apply Hfg.
-    - intros n; split.
-      + by intros f x.
-      + by intros f g ? x.
-      + by intros f g h ?? x; trans (g x).
-    - by intros n f g ? x; apply dist_S.
-  Qed.
-  Canonical Structure iprodC := OfeT (iprod B) iprod_ofe_mixin.
-
-  Program Definition iprod_chain `(c : chain iprodC)
-    (x : A) : chain (B x) := {| chain_car n := c n x |}.
-  Next Obligation. intros c x n i ?. by apply (chain_cauchy c). Qed.
-  Global Program Instance iprod_cofe `{∀ x, Cofe (B x)} : Cofe iprodC :=
-    { compl c x := compl (iprod_chain c x) }.
-  Next Obligation. intros ? n c x. apply (conv_compl n (iprod_chain c x)). Qed.
-End iprod.
-
-Arguments iprodC {_} _.
-Notation "A -c> B" :=
-  (@iprodC A (λ _, B)) (at level 99, B at level 200, right associativity).
-Instance iprod_inhabited {A} {B : A → ofeT} `{∀ x, Inhabited (B x)} :
-  Inhabited (iprodC B) := populate (λ _, inhabitant).
-
 (** Non-expansive function space *)
 Record ofe_mor (A B : ofeT) : Type := CofeMor {
   ofe_mor_car :> A → B;
@@ -761,58 +725,6 @@ Proof.
   intros ?? A1 A2 B1 B2 n ???;
     by apply prodC_map_ne; apply cFunctor_contractive.
 Qed.
-
-Definition iprod_map {A} {B1 B2 : A → ofeT} (f : ∀ x, B1 x → B2 x)
-  (g : iprod B1) : iprod B2 := λ x, f _ (g x).
-
-Lemma iprod_map_ext {A} {B1 B2 : A → ofeT} (f1 f2 : ∀ x, B1 x → B2 x)
-  (g : iprod B1) :
-  (∀ x, f1 x (g x) ≡ f2 x (g x)) → iprod_map f1 g ≡ iprod_map f2 g.
-Proof. done. Qed.
-Lemma iprod_map_id {A} {B : A → ofeT} (g : iprod B) :
-  iprod_map (λ _, id) g = g.
-Proof. done. Qed.
-Lemma iprod_map_compose {A} {B1 B2 B3 : A → ofeT}
-    (f1 : ∀ x, B1 x → B2 x) (f2 : ∀ x, B2 x → B3 x) (g : iprod B1) :
-  iprod_map (λ x, f2 x ∘ f1 x) g = iprod_map f2 (iprod_map f1 g).
-Proof. done. Qed.
-
-Instance iprod_map_ne {A} {B1 B2 : A → ofeT} (f : ∀ x, B1 x → B2 x) n :
-  (∀ x, Proper (dist n ==> dist n) (f x)) →
-  Proper (dist n ==> dist n) (iprod_map f).
-Proof. by intros ? y1 y2 Hy x; rewrite /iprod_map (Hy x). Qed.
-
-Definition iprodC_map {A} {B1 B2 : A → ofeT} (f : iprod (λ x, B1 x -n> B2 x)) :
-  iprodC B1 -n> iprodC B2 := CofeMor (iprod_map f).
-Instance iprodC_map_ne {A} {B1 B2 : A → ofeT} :
-  NonExpansive (@iprodC_map A B1 B2).
-Proof. intros n f1 f2 Hf g x; apply Hf. Qed.
-
-Program Definition iprodCF {C} (F : C → cFunctor) : cFunctor := {|
-  cFunctor_car A B := iprodC (λ c, cFunctor_car (F c) A B);
-  cFunctor_map A1 A2 B1 B2 fg := iprodC_map (λ c, cFunctor_map (F c) fg)
-|}.
-Next Obligation.
-  intros C F A1 A2 B1 B2 n ?? g. by apply iprodC_map_ne=>?; apply cFunctor_ne.
-Qed.
-Next Obligation.
-  intros C F A B g; simpl. rewrite -{2}(iprod_map_id g).
-  apply iprod_map_ext=> y; apply cFunctor_id.
-Qed.
-Next Obligation.
-  intros C F A1 A2 A3 B1 B2 B3 f1 f2 f1' f2' g. rewrite /= -iprod_map_compose.
-  apply iprod_map_ext=>y; apply cFunctor_compose.
-Qed.
-
-Notation "T -c> F" := (@iprodCF T%type (λ _, F%CF)) : cFunctor_scope.
-
-Instance iprodCF_contractive `{Finite C} (F : C → cFunctor) :
-  (∀ c, cFunctorContractive (F c)) → cFunctorContractive (iprodCF F).
-Proof.
-  intros ? A1 A2 B1 B2 n ?? g.
-  by apply iprodC_map_ne=>c; apply cFunctor_contractive.
-Qed.
-
 
 Program Definition ofe_morCF (F1 F2 : cFunctor) : cFunctor := {|
   cFunctor_car A B := cFunctor_car F1 B A -n> cFunctor_car F2 A B;
@@ -1173,6 +1085,106 @@ Instance laterCF_contractive F : cFunctorContractive (laterCF F).
 Proof.
   intros A1 A2 B1 B2 n fg fg' Hfg. apply laterC_map_contractive.
   destruct n as [|n]; simpl in *; first done. apply cFunctor_ne, Hfg.
+Qed.
+
+(* Dependently-typed functions *)
+(* We make [iprod] a definition so that we can register it as a canonical
+structure. *)
+Definition iprod {A} (B : A → ofeT) := ∀ x : A, B x.
+
+Section iprod.
+  Context {A : Type} {B : A → ofeT}.
+  Implicit Types f g : iprod B.
+
+  Instance iprod_equiv : Equiv (iprod B) := λ f g, ∀ x, f x ≡ g x.
+  Instance iprod_dist : Dist (iprod B) := λ n f g, ∀ x, f x ≡{n}≡ g x.
+  Definition iprod_ofe_mixin : OfeMixin (iprod B).
+  Proof.
+    split.
+    - intros f g; split; [intros Hfg n k; apply equiv_dist, Hfg|].
+      intros Hfg k; apply equiv_dist=> n; apply Hfg.
+    - intros n; split.
+      + by intros f x.
+      + by intros f g ? x.
+      + by intros f g h ?? x; trans (g x).
+    - by intros n f g ? x; apply dist_S.
+  Qed.
+  Canonical Structure iprodC := OfeT (iprod B) iprod_ofe_mixin.
+
+  Program Definition iprod_chain `(c : chain iprodC)
+    (x : A) : chain (B x) := {| chain_car n := c n x |}.
+  Next Obligation. intros c x n i ?. by apply (chain_cauchy c). Qed.
+  Global Program Instance iprod_cofe `{∀ x, Cofe (B x)} : Cofe iprodC :=
+    { compl c x := compl (iprod_chain c x) }.
+  Next Obligation. intros ? n c x. apply (conv_compl n (iprod_chain c x)). Qed.
+
+  Global Instance iprod_inhabited `{∀ x, Inhabited (B x)} : Inhabited iprodC :=
+    populate (λ _, inhabitant).
+  Global Instance iprod_lookup_discrete `{EqDecision A} f x :
+    Discrete f → Discrete (f x).
+  Proof.
+    intros Hf y ?.
+    set (g x' := if decide (x = x') is left H then eq_rect _ B y _ H else f x').
+    trans (g x).
+    { apply Hf=> x'. unfold g. by destruct (decide _) as [[]|]. }
+    unfold g. destruct (decide _) as [Hx|]; last done.
+    by rewrite (proof_irrel Hx eq_refl).
+  Qed.
+End iprod.
+
+Arguments iprodC {_} _.
+Notation "A -c> B" :=
+  (@iprodC A (λ _, B)) (at level 99, B at level 200, right associativity).
+
+Definition iprod_map {A} {B1 B2 : A → ofeT} (f : ∀ x, B1 x → B2 x)
+  (g : iprod B1) : iprod B2 := λ x, f _ (g x).
+
+Lemma iprod_map_ext {A} {B1 B2 : A → ofeT} (f1 f2 : ∀ x, B1 x → B2 x)
+  (g : iprod B1) :
+  (∀ x, f1 x (g x) ≡ f2 x (g x)) → iprod_map f1 g ≡ iprod_map f2 g.
+Proof. done. Qed.
+Lemma iprod_map_id {A} {B : A → ofeT} (g : iprod B) :
+  iprod_map (λ _, id) g = g.
+Proof. done. Qed.
+Lemma iprod_map_compose {A} {B1 B2 B3 : A → ofeT}
+    (f1 : ∀ x, B1 x → B2 x) (f2 : ∀ x, B2 x → B3 x) (g : iprod B1) :
+  iprod_map (λ x, f2 x ∘ f1 x) g = iprod_map f2 (iprod_map f1 g).
+Proof. done. Qed.
+
+Instance iprod_map_ne {A} {B1 B2 : A → ofeT} (f : ∀ x, B1 x → B2 x) n :
+  (∀ x, Proper (dist n ==> dist n) (f x)) →
+  Proper (dist n ==> dist n) (iprod_map f).
+Proof. by intros ? y1 y2 Hy x; rewrite /iprod_map (Hy x). Qed.
+
+Definition iprodC_map {A} {B1 B2 : A → ofeT} (f : iprod (λ x, B1 x -n> B2 x)) :
+  iprodC B1 -n> iprodC B2 := CofeMor (iprod_map f).
+Instance iprodC_map_ne {A} {B1 B2 : A → ofeT} :
+  NonExpansive (@iprodC_map A B1 B2).
+Proof. intros n f1 f2 Hf g x; apply Hf. Qed.
+
+Program Definition iprodCF {C} (F : C → cFunctor) : cFunctor := {|
+  cFunctor_car A B := iprodC (λ c, cFunctor_car (F c) A B);
+  cFunctor_map A1 A2 B1 B2 fg := iprodC_map (λ c, cFunctor_map (F c) fg)
+|}.
+Next Obligation.
+  intros C F A1 A2 B1 B2 n ?? g. by apply iprodC_map_ne=>?; apply cFunctor_ne.
+Qed.
+Next Obligation.
+  intros C F A B g; simpl. rewrite -{2}(iprod_map_id g).
+  apply iprod_map_ext=> y; apply cFunctor_id.
+Qed.
+Next Obligation.
+  intros C F A1 A2 A3 B1 B2 B3 f1 f2 f1' f2' g. rewrite /= -iprod_map_compose.
+  apply iprod_map_ext=>y; apply cFunctor_compose.
+Qed.
+
+Notation "T -c> F" := (@iprodCF T%type (λ _, F%CF)) : cFunctor_scope.
+
+Instance iprodCF_contractive `{Finite C} (F : C → cFunctor) :
+  (∀ c, cFunctorContractive (F c)) → cFunctorContractive (iprodCF F).
+Proof.
+  intros ? A1 A2 B1 B2 n ?? g.
+  by apply iprodC_map_ne=>c; apply cFunctor_contractive.
 Qed.
 
 (** Constructing isomorphic OFEs *)
